Advance proof for quantifiers, document equivalence definition

WarblreEquiv/FunctTreeCompute/EquivDef.v
@@ -6,13 +6,21 @@ Import Notation.
 Section EquivDef.
   Context `{characterClass: Character.class}.
 
+  (* Definition of when a MatcherContinuation performs a given list of actions. *)
+  (* A MatcherContinuation mc, working on input string str0 and with the open group list gl,
+  performs the actions described in act in the direction dir when: *)
   Definition equiv_cont (mc: MatcherContinuation) (gl: open_groups) (act: actions) (dir: Direction) (str0: string): Prop :=
     forall (gm: group_map) (ms: MatchState) (inp: input) (res: option MatchState) (fuel: nat) (t: tree),
+      (* for all corresponding tuples of a MatchState ms, an input inp, a group map gm 
+      and a list of open groups gl that use the input string str0, *)
       input_compat inp str0 ->
       equiv_groupmap_ms gm ms -> group_map_equiv_open_groups gm gl ->
       ms_matches_inp ms inp ->
+      (* if the continuation mc called on ms yields the result res, *)
       mc ms = Success res ->
+      (* then letting t be the tree corresponding to the actions in act on the input inp with group map gm and direction dir, *)
       compute_tree' act inp gm dir fuel = Some t ->
+      (* the first branch of t is equivalent to the result res. *)
       equiv_groupmap_ms_opt (tree_res t gm (idx inp) dir) res.
 
   Definition equiv_matcher (m: Matcher) (reg: regex) (dir: Direction): Prop :=
